% !TeX spellcheck = en_GB
\documentclass[letterpaper,12pt]{article}
\usepackage{textcomp}
\usepackage{parskip}
\usepackage{amsmath}
\usepackage{amssymb}
\usepackage{mathrsfs}
\usepackage{gensymb}
\usepackage{enumerate}
\usepackage{fullpage}
\usepackage{setspace}
\onehalfspacing

\setlength{\parindent}{0pt}
\newcommand{\vect}[1]{\mathbf{#1}}
\newcommand*\conj[1]{\bar{#1}}


\begin{document}

\textbf{\large Problem Set 4}

Natasha Watkins

\vspace{5mm}

\textbf{Exercise 1}

\begin{align*}
\frac{1}{e^{z_t}K_t^\alpha - Ae^{z_t}K_t^\alpha} &=
\beta E_t \frac{\alpha e^{z_{t+1}} (Ae^{z_t}K_t^\alpha)^{\alpha-1} } {e^{z_{t+1}} (Ae^{z_t}K_t^\alpha)^\alpha - Ae^{z_{t+1}}(Ae^{z_t}K_t^\alpha)^\alpha} \\
&= 
\beta E_t \frac{\alpha  (Ae^{z_t}K_t^\alpha)^{-1}}{ 1 - A} \\
\frac{1}{e^{z_t}K_t^\alpha(1 - A)}
&= 
\beta E_t \frac{\alpha  (Ae^{z_t}K_t^\alpha)^{-1}}{ 1 - A} \\
A
&= 
\beta \alpha
\end{align*}
Therefore,
$K_{t+1} = \beta \alpha e^{z_t} K_t^\alpha$

\textbf{Exercise 2}

\begin{enumerate}
	\item $c_t = (1 - \tau)[w_t l_t (r_t - \delta) k_t] + k_t + T_t - k_{t+1}$
	\item $\frac{1}{c_t} = \beta E_t \{\frac{1}{c_{t+1}} [(r_{t+1} - \delta)(1 - \tau) + 1]\}$
	\item $\frac{a}{1 - l_t} = \frac{1}{c_t} w_t (1 - \tau)$
	\item $r_t = \alpha e^{z_t} K_t^{\alpha - 1} L_t^{1 - \alpha}$
	\item $w_t = (1 - \alpha) e^{z_t} K_t^\alpha L_t^{-\alpha}$
	\item $\tau[w_t l_t + (r_t - \delta) k_t] = T_t$
	\item $z_t = (1 - \rho_z) \bar{z} + \rho_z z_{t-1} + \epsilon_t^z; \ \epsilon_t^z \sim i.i.d.(0, \sigma_z^2)$
\end{enumerate}

\textbf{Exercise 3}

\begin{enumerate}
	\item $c_t = (1 - \tau)[w_t l_t (r_t - \delta) k_t] + k_t + T_t - k_{t+1}$
	\item $c_t^{-\gamma} = \beta E_t \{c_{t+1}^{-\gamma} [(r_{t+1} - \delta)(1 - \tau) + 1]\}$
	\item $\frac{a}{1 - l_t} = c_t^{-\gamma} w_t (1 - \tau)$
	\item $r_t = \alpha e^{z_t} K_t^{\alpha - 1} L_t^{1 - \alpha}$
	\item $w_t = (1 - \alpha) e^{z_t} K_t^\alpha L_t^{-\alpha}$
	\item $\tau[w_t l_t + (r_t - \delta) k_t] = T_t$
	\item $z_t = (1 - \rho_z) \bar{z} + \rho_z z_{t-1} + \epsilon_t^z; \ \epsilon_t^z \sim i.i.d.(0, \sigma_z^2)$
\end{enumerate}

\textbf{Exercise 4}

\begin{enumerate}
	\item $c_t = (1 - \tau)[w_t l_t (r_t - \delta) k_t] + k_t + T_t - k_{t+1}$
	\item $c_t^{-\gamma} = \beta E_t \{c_{t+1}^{-\gamma} [(r_{t+1} - \delta)(1 - \tau) + 1]\}$
	\item $a (1 - l_t)^{-\xi} = c_t^{-\gamma} w_t (1 - \tau)$
	\item $r_t = \alpha e^{z_t} K_t^{\eta - 1} [\alpha K_t^\eta + (1 - \alpha) L_t^\eta]^{\frac{1-n}{n}}$
	\item $w_t = (1 - \alpha) e^{z_t} L_t^{\eta - 1}[\alpha K_t^\eta + (1 - \alpha)L_t^\eta]^{\frac{1-n}{n}}$
	\item $\tau[w_t l_t + (r_t - \delta) k_t] = T_t$
	\item $z_t = (1 - \rho_z) \bar{z} + \rho_z z_{t-1} + \epsilon_t^z; \ \epsilon_t^z \sim i.i.d.(0, \sigma_z^2)$
\end{enumerate}

\textbf{Exercise 5}

\begin{enumerate}
	\item $c_t = (1 - \tau)[w_t (r_t - \delta) k_t] + k_t + T_t - k_{t+1}$
	\item $c_t^{-\gamma} = \beta E_t \{c_{t+1}^{-\gamma} [(r_{t+1} - \delta)(1 - \tau) + 1]\}$
	\item $r_t = \alpha K_t^{\alpha-1} (e^{z_t})^{(1 - \alpha)}$
	\item $w_t = (1 - \alpha) K_t^\alpha (e^{z_t}) ^{-\alpha}$
	\item $\tau[w_t + (r_t - \delta) k_t] = T_t$
	\item $z_t = (1 - \rho_z) \bar{z} + \rho_z z_{t-1} + \epsilon_t^z; \ \epsilon_t^z \sim i.i.d.(0, \sigma_z^2)$
\end{enumerate}

Steady-state versions of these equations are given by
\begin{enumerate}
	\item $\bar{c} = (1 - \tau)[\bar{w} (\bar{r} - \delta) \bar{k}]  + \bar{T} $
	\item $\bar{c}^{-\gamma} = \beta E_t \{\bar{c}^{-\gamma} [(\bar{r} - \delta)(1 - \tau) + 1]\}$
	\item $\bar{r} = \alpha \bar{k}^{\alpha-1} (e^{\bar{z}})^{(1 - \alpha)}$
	\item $\bar{w} = (1 - \alpha) \bar{k}^\alpha (e^{\bar{z}}) ^{-\alpha}$
	\item $\tau[\bar{w} + (\bar{r} - \delta) \bar{k}] = \bar{T}$
	\item $0 = \epsilon_t^{\bar{z}}; \ \epsilon_t^z \sim i.i.d.(0, \sigma_z^2)$
\end{enumerate}

The algebraic solution of steady state capital as a function of $\bar{z}$ is
\begin{align*}
\bar{k} = 
\Big[ \frac{1}{(e^{\bar{z}})^{1-\alpha}} \Big( \frac{1-\beta}{\alpha\beta(1-\tau)} + \frac{\delta}{\alpha} \Big) \Big] ^{\frac{1}{\alpha - 1}}
\end{align*}

\textbf{Exercise 6}

\begin{enumerate}
	\item $c_t = (1 - \tau)[w_t (r_t - \delta) k_t] + k_t + T_t - k_{t+1}$
	\item $c_t^{-\gamma} = \beta E_t \{c_{t+1}^{-\gamma} [(r_{t+1} - \delta)(1 - \tau) + 1]\}$
	\item $a(1-l_t)^{-\xi} = c^{-\gamma} w_t (1 - \tau)$
	\item $r_t = \alpha K_t^{\alpha-1} (L_t e^{z_t})^{(1 - \alpha)}$
	\item $w_t = (1 - \alpha) K_t^\alpha (L_t e^{z_t}) ^{-\alpha}$
	\item $\tau[w_t l_t + (r_t - \delta) k_t] = T_t$
	\item $z_t = (1 - \rho_z) \bar{z} + \rho_z z_{t-1} + \epsilon_t^z; \ \epsilon_t^z \sim i.i.d.(0, \sigma_z^2)$
\end{enumerate}

Steady-state versions of these equations are given by
\begin{enumerate}
	\item $\bar{c} = (1 - \tau)[\bar{w} (\bar{r} - \delta) \bar{k}]  + \bar{T} $
	\item $\bar{c}^{-\gamma} = \beta E_t \{\bar{c}^{-\gamma} [(\bar{r} - \delta)(1 - \tau) + 1]\}$
	\item $a(1-\bar{l})^{-\xi} = c^{-\gamma} \bar{w} (1 - \tau)$
	\item $\bar{r} = \alpha \bar{k}^{\alpha-1} (\bar{l} 1 - e^{\bar{z}})^{(1 - \alpha)}$
	\item $\bar{w} = (1 - \alpha) \bar{k}^\alpha (\bar{l} e^{\bar{z}}) ^{-\alpha}$
	\item $\tau[\bar{w} \bar{l} + (\bar{r} - \delta) \bar{k}] = \bar{T}$
	\item $0 = \epsilon_t^{\bar{z}}; \ \epsilon_t^z \sim i.i.d.(0, \sigma_z^2)$
\end{enumerate}
\end{document}