\documentclass[letterpaper,12pt]{article}
\usepackage{textcomp}
\usepackage{parskip}
\usepackage{amsmath}
\usepackage{amssymb}
\usepackage{mathrsfs}
\usepackage{gensymb}
\usepackage{enumerate}
\usepackage{fullpage}
\usepackage{setspace}
\onehalfspacing

\setlength{\parindent}{0pt}
\newcommand{\vect}[1]{\mathbf{#1}}
\newcommand*\conj[1]{\bar{#1}}


\begin{document}

\textbf{\large Problem Set 2}

Natasha Watkins

\vspace{5mm}

\textbf{Exercise 4.4}

By 4.3, the characteristic polynomial of $A^H = A$ is
$$
p(\lambda) = \lambda^2 - tr(A) \lambda + \det(A)
$$
where A is a $2 \times 2$ matrix of the form
$$
A =
\begin{bmatrix}
a & b \\
c & d \\
\end{bmatrix}
$$
The diagonal elements of a Hermitian matrix are real. So the diagonal elements of $A$ are also real. We can check that the roots of the characteristic polynomial are real by finding the discriminant.
\begin{align*}
[tr(A)]^2 - 4 \det(A) &= (a + d)^2 - 4 (ad - bc) \\
&= a^2 + 2ad + d^2 -4ad + 4bc \\
&= a^2 - 4ad + d^2 + 4bc \\
&= (a - d)^2 + 4bc
\end{align*}

\underline{Part i)}

As $A^H$ is Hermitian, $b = \bar{c}$, so $4bc \geq 0$. Therefore the discriminant is positive and the roots are real.

\underline{Part ii)}

If $A^H = -A$, then $b = -\bar{c}$, so $4bc \leq 0$. Therefore, the discriminant is negative and the roots are imaginary.

\textbf{Exercise 4.6}

Consider a matrix $A$ that is upper triangular. We know that the determinant of an upper triangular matrix is the product of its diagonal elements, ie. $\det(A) = \prod_{i=1}^n a_{ii}$.

The eigenvalues of a matrix are such that $\det(\lambda I - A) = 0$.

Therefore, 
\begin{align*}
\det(\lambda I - A) &= \prod_{i=1}^n (\lambda_i - a_{ii}) = 0 \\
&= (\lambda_1 - a_{11}) \cdot (\lambda_2 - a_{22}) \cdots (\lambda_n - a_{nn}) = 0
\end{align*}
The roots of the characteristic polynomial (ie. the eigenvalues) are given by the diagonal elements of $A$.

\textbf{Exercise 4.13}

Solving for the spectrum of $A$ gives $\sigma(A) = \{\frac{2}{5}, 1 \}$, with corresponding eigenvectors of $[1, -1]^T$ and $[2, 1]^T$. Let $P$ be the transition matrix, where
\begin{align*}
P =
\begin{bmatrix}
1 & 1 \\
-1 & 2 \\
\end{bmatrix},
\quad
D =
\begin{bmatrix}
\frac{2}{5} & 0 \\
0 & 1 \\
\end{bmatrix},
\quad
P^{-1} = \frac{1}{3}
\begin{bmatrix}
1 & 1 \\
-2 & 1 \\
\end{bmatrix}
\end{align*}
Solving $P^{-1}AP$ gives
\begin{align*}
\begin{bmatrix}
	1 & 1 \\
	-1 & 2 \\
\end{bmatrix}
\begin{bmatrix}
	0.8 & 0.4 \\
	0,2 & 0.6 \\
\end{bmatrix}
\frac{1}{3}
\begin{bmatrix}
	1 & 1 \\
	-2 & 1 \\
\end{bmatrix}
=
\begin{bmatrix}
\frac{2}{5} & 0 \\
0 & 1
\end{bmatrix}
= D
\end{align*}

\textbf{Exercise 4.18}

We know that $\lambda$ satisfies $A\vect{x} = \lambda \vect{x}$ for some $\vect{x}$. Taking the transpose, we see $\vect{x}^TA^T = \lambda \vect{x}^T$. This is equivalent to $\det(A^T - \lambda I) = 0$.

The determinant of a matrix $A$ is equal to the determinant of its transpose, so
\begin{align*}
\det(A^T - \lambda I) = \det(A - \lambda I) = 0
\end{align*}
As we know $\det(A - \lambda I) = 0$ holds for some $\vect{x}$, there exists a vector $\vect{x}^T$ such that $\det(A^T - \lambda I) = 0$ holds.

\textbf{Exercise 4.20}

If $A^H$ and B are orthornormally similar, then there is $U$ such that $B = U^HA^HU$.
\begin{align*}
B^H = (U^HA^HU)^H = U^H A U = U^H A^H U = B
\end{align*}
Therefore, $B$ is also Hermitian.

\textbf{Exercise 4.27}

$A$ is a positive definite matrix, so it is Hermitian. The diagonal elements of a Hermitian matrix are real, as they are their own complex conjugate.

It also is true that $\langle \vect{x},  A\vect{x} \rangle = \vect{x}^H A \vect{x} > 0$ for any vector $\vect{x}$. Consider the vector $e_1 = [1 \ 0 \ 0 \ \cdots \ 0]^T$. $e_1^H A e_1$ selects the first diagonal element of $A$. Likewise, the vector $e_2$ selects the second diagonal element of $A$. As $A\vect{x} \rangle = \vect{x}^H A \vect{x} > 0$ holds for all vectors, the diagonal elements are all positive.

\textbf{Exercise 3.38}

\begin{enumerate}[i)]
	\item $AA^{\dagger}A = U_1 \Sigma_1 V_1^H V_1 \Sigma_1^{-1} U_1^H U_1 \Sigma_1 V_1^H = U_1  \Sigma_1 V_1^H = A $
	\item $A^{\dagger} A A^{\dagger} = V_1 \Sigma_1^{-1} U_1^H U_1 \Sigma_1 V_1^H V_1 \Sigma_1^{-1} U_1^H =  V_1 \Sigma_1^{-1} U_1^H = A^{\dagger}$
	\item $(A A^{\dagger})^H = ((V_1 \Sigma_1 U_1^H) (U_1 \Sigma_1^{-1} V_1^H))^H = V_1 \Sigma_1^{-1} U_1^H U_1 \Sigma_1 V_1^H = A^{\dagger} A$
	\item $(A^{\dagger} A)^H = (( V_1 \Sigma_1^{-1} U_1^H)(U_1 \Sigma_1 V_1^H))^H = V_1 \Sigma_1 U_1^H U_1 \Sigma_1^{-1} V_1^H = V_1 V_1^H = A^{\dagger} A$
\end{enumerate}

\end{document}